Break dependency of Slabs2 on Slabs

src/SlabsCommon.fst
@@ -126,7 +126,6 @@ let p_empty_pack (#opened:_)
     (fun x y -> x == y)
     (fun _ -> ())
 
-
 let p_partial_pack (#opened:_)
   (sc: sc)
   (b1: blob)
@@ -532,4 +531,71 @@ let pack_slab_starseq
     (SeqUtils.init_u32_refined (U32.v md_count_v))
     (SeqUtils.init_u32_refined (U32.v md_count_v))
     (US.v idx)
+#pop-options
+
+#push-options "--z3rlimit 20 --compat_pre_typed_indexed_effects"
+let pack_right_and_refactor_vrefine_dep
+  (#opened:_)
+  (size_class: sc)
+  (slab_region: array U8.t{A.length slab_region = U32.v metadata_max * U32.v page_size})
+  (md_bm_region: array U64.t{A.length md_bm_region = U32.v metadata_max * 4})
+  (md_region: array AL.cell{A.length md_region = U32.v metadata_max})
+  (md_count: ref U32.t)
+  (r1 r2 r3: ref US.t)
+  (md_count_v: U32.t{U32.v md_count_v <= U32.v metadata_max})
+  : SteelGhost unit opened
+  (
+    vrefinedep
+      (vptr md_count)
+      vrefinedep_prop
+      (left_vprop size_class (A.split_r slab_region 0sz) md_bm_region md_region r1 r2 r3)
+    `star`
+    (right_vprop (A.split_r slab_region 0sz) md_bm_region md_region md_count_v `star`
+    A.varray (A.split_l slab_region 0sz))
+  )
+  (fun _ ->
+    vrefinedep
+      (vptr md_count)
+      vrefinedep_prop
+      (size_class_vprop_aux size_class slab_region md_bm_region md_region r1 r2 r3)
+  )
+  (requires fun h0 ->
+    let blob0
+      = h0 (vrefinedep
+      (vptr md_count)
+      vrefinedep_prop
+      (left_vprop size_class (A.split_r slab_region 0sz) md_bm_region md_region r1 r2 r3)
+    ) in
+    md_count_v == dfst blob0)
+  (ensures fun h0 _ h1 ->
+    let blob0
+      = h0 (vrefinedep
+      (vptr md_count)
+      vrefinedep_prop
+      (left_vprop size_class (A.split_r slab_region 0sz) md_bm_region md_region r1 r2 r3)
+    ) in
+    let blob1
+      = h1 (vrefinedep
+      (vptr md_count)
+      vrefinedep_prop
+      (size_class_vprop_aux size_class slab_region md_bm_region md_region r1 r2 r3)
+    ) in
+    dfst blob0 == dfst blob1
+  )
+  =
+  let md_count_v' = elim_vrefinedep
+    (vptr md_count)
+    vrefinedep_prop
+    (left_vprop size_class (A.split_r slab_region 0sz) md_bm_region md_region r1 r2 r3) in
+  assert (G.reveal md_count_v' == md_count_v);
+  change_equal_slprop
+    (right_vprop (A.split_r slab_region 0sz) md_bm_region md_region md_count_v)
+    (right_vprop (A.split_r slab_region 0sz) md_bm_region md_region (G.reveal md_count_v'));
+  intro_vrefinedep
+    (vptr md_count)
+    vrefinedep_prop
+    (size_class_vprop_aux size_class slab_region md_bm_region md_region r1 r2 r3)
+    (left_vprop size_class (A.split_r slab_region 0sz) md_bm_region md_region r1 r2 r3 (G.reveal md_count_v') `star`
+    right_vprop (A.split_r slab_region 0sz) md_bm_region md_region (G.reveal md_count_v') `star`
+    A.varray (A.split_l slab_region 0sz))
 #pop-options
